Dead End: Clean up Reaction(M) parameters

Runtime/Reaction.lean
@@ -2,42 +2,74 @@ import Runtime.Time
 import Runtime.Interface
 import Runtime.Utilities
 
-structure Reaction.Event (σAction : Interface.Scheme) (min : Time) where 
+-- NOTE: This approach doesn't work unfortunately: https://leanprover.zulipchat.com/#narrow/stream/270676-lean4/topic/Type.20Inference.20Problem
+
+namespace ReactionM
+
+structure Event (σAction : Interface.Scheme) (min : Time) where 
   action : σAction.vars
   value  : σAction.type action
   time   : Time.From min
 
-instance : LE (Reaction.Event σAction time) where
+instance : LE (Event σAction time) where
   le e₁ e₂ := e₁.time ≤ e₂.time
 
-instance : Decidable ((e₁ : Reaction.Event σAction time) ≤ e₂) := by
+instance : Decidable ((e₁ : Event σAction time) ≤ e₂) := by
   simp [LE.le]; infer_instance
 
-namespace ReactionM
-open Reaction
+structure Input.Schemes where
+  portSource   : Interface.Scheme
+  actionSource : Interface.Scheme
+  state        : Interface.Scheme
+  param        : Interface.Scheme
 
-structure Input (σPortSource σActionSource σState σParam : Interface.Scheme) where
-  ports          : Interface? σPortSource
-  actions        : Interface? σActionSource
-  state          : Interface σState
-  params         : Interface σParam
+open Input.Schemes in attribute [reducible] portSource actionSource state param
+
+structure Input (σs : Input.Schemes) where
+  ports          : Interface? σs.portSource
+  actions        : Interface? σs.actionSource
+  state          : Interface σs.state
+  params         : Interface σs.param
   tag            : Tag
   physicalOffset : Duration
 
-structure Output (σPortEffect σActionEffect σState : Interface.Scheme) (min : Time) where
-  ports  : Interface? σPortEffect := Interface?.empty
-  state  : Interface σState
-  events : SortedArray (Event σActionEffect min) := #[]#
+structure Output.Schemes where
+  portEffect   : Interface.Scheme
+  actionEffect : Interface.Scheme
+  state        : Interface.Scheme
 
-def _root_.ReactionT (σPortSource σPortEffect σActionSource σActionEffect σState σParam : Interface.Scheme) (m : Type → Type) (α : Type) := 
-  (input : Input σPortSource σActionSource σState σParam) → m (Output σPortEffect σActionEffect σState input.tag.time × α)
+open Output.Schemes in attribute [reducible] portEffect actionEffect state
 
-def _root_.ReactionM (σPortSource σPortEffect σActionSource σActionEffect σState σParam : Interface.Scheme) := 
-  ReactionT σPortSource σPortEffect σActionSource σActionEffect σState σParam IO
+structure Output (σs : Output.Schemes) (min : Time) where
+  ports  : Interface? σs.portEffect := Interface?.empty
+  state  : Interface σs.state
+  events : SortedArray (Event σs.actionEffect min) := #[]#
 
-variable {σInput σOutput σAction σPortSource σPortEffect σActionSource σActionEffect σState σParam : Interface.Scheme} 
+structure Schemes where
+  portSource   : Interface.Scheme
+  portEffect   : Interface.Scheme
+  actionSource : Interface.Scheme
+  actionEffect : Interface.Scheme
+  state        : Interface.Scheme
+  param        : Interface.Scheme
 
-def Output.merge (o₁ o₂ : ReactionM.Output σPortEffect σActionEffect σState time) : Output σPortEffect σActionEffect σState time where
+open Schemes in attribute [reducible] portSource portEffect actionSource actionEffect state param
+
+abbrev Schemes.inputSchemes (σs : Schemes) : Input.Schemes where
+  portSource   := σs.portSource
+  actionSource := σs.actionSource
+  state        := σs.state
+  param        := σs.param
+
+abbrev Schemes.outputSchemes (σs : Schemes) : Output.Schemes where
+  portEffect   := σs.portEffect
+  actionEffect := σs.actionEffect
+  state        := σs.state
+
+abbrev _root_.ReactionM (σs : Schemes) (α : Type) := 
+  (input : Input σs.inputSchemes) → IO (Output σs.outputSchemes input.tag.time × α)
+
+def Output.merge (o₁ o₂ : ReactionM.Output σs time) : Output σs time where
   ports  := o₁.ports.merge o₂.ports
   state  := o₂.state
   events := o₁.events.merge o₂.events
@@ -51,14 +83,15 @@ theorem Output.merge_state : (Output.merge o₁ o₂).state = o₂.state := rfl
 @[simp]
 theorem Output.merge_events : (Output.merge o₁ o₂).events = o₁.events.merge o₂.events := rfl
 
-def Input.noop (input : Input σPortSource σActionSource σState σParam) : Output σPortEffect σActionEffect σState input.tag.time where 
+def Input.noop (input : Input σsᵢ) : Output ⟨σPortEffect, σActionEffect, σsᵢ.state⟩ input.tag.time where 
   state := input.state 
 
 @[simp]
-theorem Input.noop_ports_isEmpty (input : Input σPortSource σActionSource σState σParam) {σPortEffect σActionEffect} : 
-  input.noop (σPortEffect := σPortEffect) (σActionEffect := σActionEffect) |>.ports.isEmpty := rfl
+theorem Input.noop_ports_isEmpty (input : Input σs) : 
+  input.noop (σPortEffect := σPortEffect) (σActionEffect := σActionEffect) |>.ports.isEmpty := 
+  rfl
 
-instance : Monad (ReactionM σPortSource σPortEffect σActionSource σActionEffect σState σParam) where
+instance : Monad (ReactionM σs) where
   pure a input := do
     let output := input.noop
     return (output, a)
@@ -77,17 +110,19 @@ instance : Monad (ReactionM σPortSource σPortEffect σActionSource σActionEff
     let output := output₁.merge output₂
     return (output, b)
 
-instance : LawfulMonad (ReactionM σPortSource σPortEffect σActionSource σActionEffect σState σParam) :=
+instance : LawfulMonad (ReactionM σs) :=
   sorry -- https://github.com/leanprover/std4/blob/23f8577169c049e6eb472a0354c11b9b934b4282/Std/Classes/LawfulMonad.lean#L12
 
-instance : MonadLift IO (ReactionM σPortSource σPortEffect σActionSource σActionEffect σState σParam) where
+instance : MonadLift IO (ReactionM σs) where
   monadLift io input world := 
     match io world with 
     | .error e world' => .error e world'
     | .ok    a world' => .ok (input.noop, a) world'
 
-def getInput (port : σPortSource.vars) : ReactionM σPortSource σPortEffect σActionSource σActionEffect σState σParam (Option $ σPortSource.type port) :=
-  fun input => return (input.noop, input.ports port)
+variable {σs : Schemes} 
+
+def getInput (port : σs.portSource.vars) : ReactionM σs (Option <| σs.portSource.type port) := fun input => 
+  return (input.noop, input.ports port)
 
 /-
 -- https://github.com/leanprover/std4/blob/23f8577169c049e6eb472a0354c11b9b934b4282/Std/Classes/LawfulMonad.lean#L69
@@ -97,61 +132,56 @@ theorem getInput_def (input : Input σPortSource σActionSource σState σParam)
   := sorry
 -/
 
-def getState (stv : σState.vars) : ReactionM σPortSource σPortEffect σActionSource σActionEffect σState σParam (σState.type stv) :=
-  fun input => return (input.noop, input.state stv)
+def getState (stv : σs.state.vars) : ReactionM σs (σs.state.type stv) := fun input => 
+  return (input.noop, input.state stv)
 
-def getAction (action : σActionSource.vars) : ReactionM σPortSource σPortEffect σActionSource σActionEffect σState σParam (Option $ σActionSource.type action) :=
-  fun input => return (input.noop, input.actions action)
+def getAction (action : σs.actionSource.vars) : ReactionM σs (Option <| σs.actionSource.type action) := fun input => 
+  return (input.noop, input.actions action)
 
-def getParam (param : σParam.vars) : ReactionM σPortSource σPortEffect σActionSource σActionEffect σState σParam (σParam.type param) :=
-  fun input => return (input.noop, input.params param)
+def getParam (param : σs.param.vars) : ReactionM σs (σs.param.type param) := fun input => 
+  return (input.noop, input.params param)
 
-def getTag : ReactionM σPortSource σPortEffect σActionSource σActionEffect σState σParam Tag := 
-  fun input => return (input.noop, input.tag)
+def getTag : ReactionM σs Tag := fun input => 
+  return (input.noop, input.tag)
 
-def getLogicalTime : ReactionM σPortSource σPortEffect σActionSource σActionEffect σState σParam Time := 
-  return (← getTag).time
+def getLogicalTime : ReactionM σs Time := fun input => 
+  return (input.noop, input.tag.time)
 
-def getPhysicalTime : ReactionM σPortSource σPortEffect σActionSource σActionEffect σState σParam Time :=
-  fun input => return (input.noop, (← Time.now) - input.physicalOffset)
+def getPhysicalTime : ReactionM σs Time := fun input => 
+  return (input.noop, (← Time.now) - input.physicalOffset)
 
-def setOutput (port : σPortEffect.vars) (v : σPortEffect.type port) : ReactionM σPortSource σPortEffect σActionSource σActionEffect σState σParam Unit :=
+def setOutput (port : σs.portEffect.vars) (v : σs.portEffect.type port) : ReactionM σs Unit :=
   fun input => 
     let ports := fun p => if h : p = port then some (h ▸ v) else none
     let output := { ports := ports, state := input.state }
     return (output, ())
 
-def setState (stv : σState.vars) (v : σState.type stv) : ReactionM σPortSource σPortEffect σActionSource σActionEffect σState σParam Unit :=
-  fun input =>
-    let state := fun s => if h : s = stv then h ▸ v else input.state s
-    let output := { state := state }
-    return (output, ())
+def setState (stv : σs.state.vars) (v : σs.state.type stv) : ReactionM σs Unit := fun input =>
+  let state := fun s => if h : s = stv then h ▸ v else input.state s
+  let output := { state := state }
+  return (output, ())
 
-def schedule (action : σActionEffect.vars) (delay : Duration) (v : σActionEffect.type action) : ReactionM σPortSource σPortEffect σActionSource σActionEffect σState σParam Unit := 
-  fun input => 
-    let time := input.tag.time.advance delay
-    let event : Event σActionEffect input.tag.time := { action := action, time := time, value := v }
-    let output := { state := input.state, events := #[event]# }
-    return (output, ())
+def schedule (action : σs.actionEffect.vars) (delay : Duration) (v : σs.actionEffect.type action) : ReactionM σs Unit := fun input => 
+  let time := input.tag.time.advance delay
+  let event := { action := action, time := time, value := v }
+  let output := { state := input.state, events := #[event]# }
+  return (output, ())
 
 end ReactionM
 
-namespace Reaction
-
-inductive Trigger (Port Action Timer : Type)
+inductive Reaction.Trigger (Port Action Timer : Type)
   | startup
   | shutdown
   | port (p : Port)
   | action (a : Action)
   | timer (t : Timer)
 
-open Reaction in
-structure _root_.Reaction (σInput σOutput σAction σState σParam : Interface.Scheme) (TimerNames : Type) where
+structure Reaction (σInput σOutput σAction σState σParam : Interface.Scheme) (TimerNames : Type) where
   portSources : Type
   portEffects : Type 
   actionSources : Type
   actionEffects : Type
-  triggers : Array (Trigger portSources actionSources TimerNames)
+  triggers : Array (Reaction.Trigger portSources actionSources TimerNames)
   [portSourcesDecEq : DecidableEq portSources]
   [portEffectsDecEq : DecidableEq portEffects]
   [actionSourcesDecEq : DecidableEq actionSources]
@@ -160,13 +190,14 @@ structure _root_.Reaction (σInput σOutput σAction σState σParam : Interface
   [portEffectsInjCoe : InjectiveCoe portEffects σOutput.vars]
   [actionSourcesInjCoe : InjectiveCoe actionSources σAction.vars]
   [actionEffectsInjCoe : InjectiveCoe actionEffects σAction.vars]
-  body : ReactionM (σInput.restrict portSources) (σOutput.restrict portEffects) (σAction.restrict actionSources) (σAction.restrict actionEffects) σState σParam Unit
+  body : ReactionM ⟨σInput.restrict portSources, σOutput.restrict portEffects, σAction.restrict actionSources, σAction.restrict actionEffects, σState, σParam⟩ Unit
 
-open Reaction in
+namespace Reaction
+
 attribute [instance] portSourcesDecEq portEffectsDecEq actionSourcesDecEq actionEffectsDecEq portSourcesInjCoe portEffectsInjCoe actionSourcesInjCoe actionEffectsInjCoe
 
 abbrev outputType (rcn : Reaction σInput σOutput σAction σState σParam TimerNames) :=
-  ReactionM.Output (σOutput.restrict rcn.portEffects) (σAction.restrict rcn.actionEffects) σState 
+  ReactionM.Output ⟨σOutput.restrict rcn.portEffects, σAction.restrict rcn.actionEffects, σState⟩
 
 def run 
   (rcn : Reaction σInput σOutput σAction σState σParam TimerNames) 
